Weidenbach_Book/IsaSAT/IsaSAT_Backtrack_LLVM.thy
@@ -154,7 +154,7 @@ lemma extract_shorter_conflict_list_heur_st_alt_def:
      ASSERT(lookup_conflict_remove1_pre (-K, D));
      let D = lookup_conflict_remove1 (-K) D;
      let outl = outl[0 := -K];
-     vm \<leftarrow> isa_vmtf_mark_to_rescore_also_reasons M N outl K vm;
+     vm \<leftarrow> isa_vmtf_mark_to_rescore_also_reasons M N outl (-K) vm;
      (D, cach, outl) \<leftarrow> isa_minimize_and_extract_highest_lookup_conflict M N D cach lbd outl;
      ASSERT(empty_cach_ref_pre cach);
      let cach = empty_cach_ref cach;
@@ -166,7 +166,8 @@ lemma extract_shorter_conflict_list_heur_st_alt_def:
   by (auto simp: the_lookup_conflict_def Let_def intro!: ext)
 
 sepref_register isa_minimize_and_extract_highest_lookup_conflict
-  empty_conflict_and_extract_clause_heur
+    empty_conflict_and_extract_clause_heur
+    isa_vmtf_mark_to_rescore_also_reasons
 
 sepref_def extract_shorter_conflict_list_heur_st_fast
   is \<open>extract_shorter_conflict_list_heur_st\<close>
@@ -178,7 +179,6 @@ sepref_def extract_shorter_conflict_list_heur_st_fast
     fold_tuple_optimizations
   apply (annot_snat_const \<open>TYPE(64)\<close>)
   by sepref
-
 
 sepref_register find_lit_of_max_level_wl
   extract_shorter_conflict_list_heur_st lit_of_hd_trail_st_heur propagate_bt_wl_D_heur
